\begin{warn}
	The following section does not use the notation of the rest of the article.
\end{warn}
With some checks out of the way, here are some actual consequences. To begin, we state Hilbert's Theorem 90.
\begin{lemma} \label{lem:hilbert90}
	Suppose that $L/K$ is a (finite) cyclic extension of fields such that $\Gamma\coloneqq\op{Gal}(L/K)$ is generated by $\sigma\in\Gamma$. Given some $\alpha\in L^\times$ such that $\op N(\alpha)=1$, there exists $\beta_0\in L^\times$ such that $\alpha=\beta_0/\sigma\beta_0$. In fact, this $\beta_0$ is unique ``up to a multiple in $K^\times$'' in the sense that
	\[\left\{\beta\in L^\times:\alpha=\beta/\sigma\beta\right\}=\left\{x\beta_0:x\in K^\times\right\}.\]
\end{lemma}
\begin{proof}
	That such a $\beta_0$ exists follows directly from Hilbert's Theorem 90. For the last sentence, of course any $\beta\coloneqq x\beta_0\in L^\times$ with $x\in K^\times$ will have
	\[\frac\beta{\sigma\beta}=\frac{\beta_0}{\sigma\beta_0}=\alpha.\]
	In the other direction, if $\beta\in L^\times$ has $\beta/\sigma\beta=\alpha$, then
	\[\sigma(\beta/\beta_0)=(\sigma\beta)/(\sigma\beta_0)=\beta/\beta_0,\]
	so $\beta/\beta_0\in K^\times$ and $\beta=(\beta/\beta_0)\cdot\beta_0$.
\end{proof}
And here are some quick consequences of this.
\begin{cor}
	Fix everything as in the set-up, and fix $\alpha\in ML^\times$ such that $\op N_{ML/L}(\alpha)=p$. Choosing some $\sigma\in\{\sigma_K,\sigma_x\}$, the elements $\eta_{\sigma}$ satisfying
	\[\frac{\eta_{\sigma}}{\sigma_K^f\left(\eta_{\sigma}\right)}=\frac{\sigma(\alpha)}{\alpha}\]
	are unique up to a multiple in $L^\times$, in the sense of \autoref{lem:hilbert90}.
\end{cor}
\begin{proof}
	Note that $\op{Gal}(ML/L)=\langle\sigma_K^f\rangle$ is cyclic generated by $\sigma_K^f$ and $\op N_{ML/L}(\sigma\alpha/\alpha)=p/p=1$, so we may simply apply \autoref{lem:hilbert90} directly to get the result.
\end{proof}
We might be worried that our choice $\alpha$ is affecting the set of $\eta_{c(\sigma_K)}$ or $\eta_{c(\sigma_x)}$, but in fact they are not, more or less.
\begin{cor} \label{cor:updatealpha}
	Fix everything as in the set-up, and choose $\sigma\in\{\sigma_K,\sigma_x\}$. Given $\alpha\in ML^\times$ such that $\op N_{ML/L}(\alpha)=p$, define
	\[S_\alpha\coloneqq\left\{\eta_\sigma\in ML^\times:\frac{\eta_{\sigma}}{\sigma_K^f\left(\eta_{\sigma}\right)}=\frac{\sigma(\alpha)}{\alpha}\right\}.\]
	Then the set $S_\alpha$ is ``unique up to a multiple in $ML^\times$'' in the sense that two $\alpha,\alpha'\in ML^\times$ with $\op N_{ML/L}(\alpha)=\op N_{ML/L}(\alpha')=p$ have some $\chi\in ML^\times$ such that
	\[S_{\alpha}=\chi\cdot S_{\alpha'}\coloneqq\{\chi\cdot \eta_\sigma:\eta_\sigma\in S_{\alpha'}\}.\]
\end{cor}
\begin{proof}
	Suppose $\alpha,\alpha'\in ML^\times$ satisfy $\op N_{ML/L}(\alpha)=\op N_{ML/L}(\alpha')=p$. The key point is that
	\[\op N_{ML/L}(\alpha/\alpha')=p/p=1,\]
	so \autoref{lem:hilbert90} promises us some $\gamma\in ML^\times$ such that $\alpha/\alpha'=\gamma/\sigma_K^f(\gamma)$. As such, we see that
	\[\frac{\sigma(\alpha)}{\alpha}=\frac{\sigma(\alpha/\alpha')}{\alpha/\alpha'}\cdot\frac{\sigma(\alpha')}{\alpha'}=\frac{(\sigma\gamma/\gamma)}{\sigma_K^f(\sigma\gamma/\gamma)}\cdot\frac{\sigma(\alpha')}{\alpha'}.\]
	As such, we set $\chi\coloneqq(\sigma\gamma/\gamma)$.
	
	To finish, we check that $S_\alpha\subseteq \chi\cdot S_{\alpha'}$, and the other inclusion is similar. Well, if $\eta_\sigma\in S_{\alpha'}$, then
	\[\frac{\chi \eta_\sigma}{\sigma_K^f(\chi \eta_\sigma)}=\frac \chi {\sigma_K^f(\chi )}\cdot\frac{\eta_\sigma}{\sigma_K^f(\eta_\sigma)}=\frac{(\sigma\gamma/\gamma)}{\sigma_K^f(\sigma\gamma/\gamma)}\cdot\frac{\sigma(\alpha')}{\alpha'}=\frac{\sigma(\alpha)}\alpha,\]
	so $\chi \eta_\sigma\in S_\alpha$. This finishes.
	% \begin{itemize}
	% 	\item We check $x\cdot S_{\alpha'}\subseteq S_\alpha$. Well, if $\eta_\sigma\in S_{\alpha'}$, then
	% 	\[\frac{x\eta_\sigma}{\sigma_K^f(x\eta_\sigma)}=\frac x{\sigma_K^f(x)}\cdot\frac{\eta_\sigma}{\sigma_K^f(\eta_\sigma)}=\frac{(\sigma\gamma/\gamma)}{\sigma_K^f(\sigma\gamma/\gamma)}\cdot\frac{\sigma(\alpha')}{\alpha'}=\frac{\sigma(\alpha)}\alpha,\]
	% 	so $x\eta_\sigma\in S_\alpha$.
	% 	\item We check $S_\alpha\subseteq x\cdot S_{\alpha'}$. Again, if $\eta_\sigma\in S_\alpha$, then
	% 	\[\frac{x^{-1}\eta_\sigma}{\sigma_K^f(x^{-1}\eta_\sigma)}=\frac {x^{-1}}{\sigma_K^f(x^{-1})}\cdot\frac{\eta_\sigma}{\sigma_K^f(\eta_\sigma)}=\left(\frac{(\sigma\gamma/\gamma)}{\sigma_K^f(\sigma\gamma/\gamma)}\right)^{-1}\cdot\frac{\sigma(\alpha)}{\alpha}=\frac{\sigma(\alpha')}{\alpha'},\]
	% 	so $\eta_\sigma=x\cdot x^{-1}\eta_\sigma\in x\cdot S_{\alpha'}$.
	% \end{itemize}
	% The above two inclusions complete the proof.
\end{proof}
We now return to describing triples.
\begin{cor} \label{cor:fullclass}
	Fix everything as in the set-up, and fix $\alpha\in ML^\times$ such that $\op N_{ML/L}(\alpha)=p$. Then, for any triple $(\alpha_1',\alpha_2',\beta')$ corresponding to the fundamental class, there exist elements $\eta_{c(\sigma_K)}',\eta_{c(\sigma_x)}'\in ML^\times$ with
	\[\frac{\eta_{c(\sigma_K)}'}{\sigma_K^f\left(\eta_{c(\sigma_K)}'\right)}=\frac{\sigma_K(\alpha)}{\alpha}\qquad\text{and}\qquad\frac{\eta_{c(\sigma_x)}'}{\sigma_K^f\left(\eta_{c(\sigma_x)}'\right)}=\frac{\sigma_x(\alpha)}{\alpha}\]
	such that
	\[(\alpha_1',\alpha_2',\beta')=\left(\alpha\cdot\prod_{i=0}^{f-1}\sigma_K^i\left(\eta_{c(\sigma_K)}'\right),\quad\prod_{i=0}^{\varphi\left(p^\nu\right)-1}\sigma_x^i\left(\eta_{c(\sigma_x)}'\right),\quad\frac{\sigma_K\left(\eta_{c(\sigma_x)}'\right)}{\eta_{c(\sigma_x)}'}\cdot\frac{\eta_{c(\sigma_K)}'}{\sigma_x\left(\eta_{c(\sigma_K)}'\right)}\right).\]
	In other words, all triples corresponding to the fundamental class come from the recipe described in \autoref{cor:fundtriple}.
\end{cor}
\begin{proof}
	By \autoref{cor:fundtriple}, we can certainly find some elements $\eta_{c(\sigma_K)},\eta_{c(\sigma_x)}\in ML^\times$ such that
	\[\frac{\eta_{c(\sigma_K)}}{\sigma_K^f\left(\eta_{c(\sigma_K)}\right)}=\frac{\sigma_K(\alpha)}{\alpha}\qquad\text{and}\qquad\frac{\eta_{c(\sigma_x)}}{\sigma_K^f\left(\eta_{c(\sigma_x)}\right)}=\frac{\sigma_x(\alpha)}{\alpha},\]
	for which
	\[(\alpha_1,\alpha_2,\beta)\coloneqq\left(\alpha\cdot\prod_{i=0}^{f-1}\sigma_K^i\left(\eta_{c(\sigma_K)}\right),\quad\prod_{i=0}^{\varphi\left(p^\nu\right)-1}\sigma_x^i\left(\eta_{c(\sigma_x)}\right),\quad\frac{\sigma_K\left(\eta_{c(\sigma_x)}\right)}{\eta_{c(\sigma_x)}}\cdot\frac{\eta_{c(\sigma_K)}}{\sigma_x\left(\eta_{c(\sigma_K)}\right)}\right)\]
	corresponds to the fundamental class $u_{L/K}\in H^2(\op{Gal}(L/K),L^\times)$. In particular, $(\alpha_1,\alpha_2,\beta)$ and $(\alpha_1',\alpha_2',\beta')$ both correspond to the same cohomology class and hence in the same equivalence class of triples, so we know that there exist $m_1,m_2\in L^\times$ such that
	\[\alpha_1'=\alpha_1\cdot\op N_{L/L_1}(m_1),\quad\alpha_2'=\alpha_2\cdot\op N_{L/L_2}(m_2),\quad\beta'=\beta\cdot\frac{\sigma_K(m_2)}{m_2}\cdot\frac{m_1}{\sigma_x(m_1)}.\]
	As such, we set $\eta_{c(\sigma_K)}'\coloneqq \eta_{c(\sigma_K)}\cdot m_1$ and $\eta_{c(\sigma_x)}'\coloneqq \eta_{c(\sigma_x)}\cdot m_2$, and these can be checked to work. For example, $\eta_{c(\sigma_K)}'$ satisfies
	\[\frac{\eta_{c(\sigma_K)}'}{\sigma_K^f\left(\eta_{c(\sigma_K)}'\right)}=\frac{\sigma_K(\alpha)}{\alpha}\qquad\text{and}\qquad\frac{\eta_{c(\sigma_x)}'}{\sigma_K^f\left(\eta_{c(\sigma_x)}'\right)}=\frac{\sigma_x(\alpha)}{\alpha}\]
	by \autoref{lem:hilbert90}. The rest of the checks are similar.
\end{proof}
\begin{corollary} \label{cor:classofa1}
	Fix everything as in the set-up, and let $\pi_1\in L_1^\times$ be a uniformizer. If the triple $(\alpha_1,\alpha_2,\beta)$ is a triple corresponding to the fundamental class, then
	\[\alpha_1\equiv\pi_1\pmod{\op N_{L/L_1}(L^\times)}.\]
\end{corollary}
\begin{proof}[Proof by triples]
	Note that $L/L_1$ is an unramified extension, so all elements of absolute value $1$ are norms, so there is in fact a class of elements containing all uniformizers in $L_1^\times/\op N_{L/L_1}(L^\times)$. Further, because $\alpha_1$ is also only defined up to a multiple in $\op N_{L/L_1}(L^\times)$, to show that the classes in $L^\times/\op N_{L/L_1}(L^\times)$ coincide, it thus suffices to exhibit a single triple $(\alpha_1,\alpha_2,\beta)$ such that $\alpha_1\in L_1^\times$ is a uniformizer.

	This is a matter of force. To begin, we can use \autoref{cor:fundtriple} to find some $\alpha$ with $\op N_{ML/L}(\alpha)=p$ and $\eta_{c(\sigma_K)},\eta_{c(\sigma_x)}\in ML^\times$ giving the triple $(\alpha_1,\alpha_2,\beta)$ as described. The idea is to force $\eta_{c(\sigma_K)}$ to have valuation zero.
	
	Let $v_{ML}$ be the fixed valuation of $ML$ extending the standard valuation $v_{\QQ_p}$ on $\QQ_p$, and let $v_{L}$ be its restriction to $L$. Because $ML/L$ is an unramified, the image of $v_{ML}$ and $v_L$ in $\QQ$ is the same. In particular, we can find some $m_1\in L_1^\times$ such that
	\[v_{ML}\left(\eta_{c(\sigma_K)}\right)=v_L(m_1).\]
	Thus, we replace $\eta_{c(\sigma_K)}$ with $\eta_{c(\sigma_K)}/m_1$, and we still satisfy the conditions of \autoref{cor:fundtriple} by \autoref{lem:hilbert90} while getting $v_{ML}\left(\eta_{c(\sigma_K)}\right)=0$. Now, the corresponding $\alpha_1$ looks like
	\[\alpha_1=\alpha\cdot\prod_{i=0}^{f-1}\sigma_K^i\left(\eta_{c(\sigma_K)}\right).\]
	In particular, defining $v_{L_1}\coloneqq v_L|_{L_1}$, it follows
	\[v_{L_1}(\alpha_1)=v_{ML}(\alpha_1)=v_{ML}(\alpha),\]
	However, $\op N_{ML/L}(\alpha)=p$ by construction, so we see that
	\[[ML:L]v_{ML}(\alpha)=v_{ML}(p)=v_{\QQ_p}(p)=1.\]
	Explicitly, we see that
	\[[ML:L]=[\QQ(\zeta_{N'}):\QQ(\zeta_m)]=\frac{[\QQ(\zeta_{N'}):\QQ_p]}{[\QQ_p(\zeta_m):\QQ_p]}=\frac nf=\varphi\left(p^\nu\right).\]
	However, $L_1/K$ has ramification degree $\varphi\left(p^\nu\right)$ (from the maximal totally ramified subextension $\QQ_p(\zeta_{p^\nu})$), so its uniformizers are the elements of valuation $1/\varphi\left(p^\nu\right)$. Thus, we have computed that $\alpha_1$ has the correct valuation and hence is a uniformizer.
\end{proof}
\begin{proof}[Proof by the Artin map]
	We take a moment to say that there is an alternate derivation of \autoref{cor:classofa1} using the Artin map: one can show that, if $u\in Z^2(L/K)$ is a representative of the fundamental class of an abelian extension $L/K$, then
	\begin{align*}
		\op{Gal}(L/K) &\to K^\times/\op N(L^\times) \\
		\sigma &\mapsto \prod_{g\in\op{Gal}(L/K)}u(g,\sigma)
	\end{align*}
	is the inverse Artin map. In particular, from our explicit formula for $\alpha_1$, we see
	\[\alpha_1=\prod_{g\in\op{Gal}(L/L_1)}u(g,\overline\sigma_K)=\theta_{L/L_1}^{-1}(\overline\sigma_K).\]
	However, $\overline\sigma_K$ is the Frobenius automorphism of $L/L_1$ because the extension $L_1/K$ is totally ramified, implying that the residue field of $L_1$ is the same as $K=\QQ_p$. Thus, $\theta_{L/L_1}^{-1}(\overline\sigma_K)$ is the class containing the uniformizers of $L_1^\times$.
\end{proof}
We close with a sanity check.
\begin{cor}
	Fix everything as in the set-up, and let $T_\alpha$ denote the set of triples $(\alpha_1,\alpha_2,\beta)$ generated by some element $\alpha\in ML^\times$ with $\op N_{ML/L}(\alpha)=p$ via \autoref{cor:fundtriple}. Then $T_\alpha$ is independent of $\alpha$.
\end{cor}
\begin{proof}
	The main idea is to use (the proof of) \autoref{cor:updatealpha}. Fix $\alpha,\alpha'\in ML^\times$ with $\op N_{ML/L}(\alpha)=\op N_{ML/L}(\alpha')=p$, and we need to show that $T_\alpha=T_{\alpha'}$. By symmetry, it will be enough for $T_\alpha\subseteq T_{\alpha'}$.

	Following the proof of \autoref{cor:updatealpha}, note that $\op N_{ML/L}(\alpha/\alpha')=1$, so we are promised $\gamma\in ML^\times$ such that $\alpha/\alpha'=\gamma/\sigma_K^f(\gamma)$. Then we showed that any $\sigma\in\{\sigma_K,\sigma_x\}$ can set
	\[\chi_\sigma\coloneqq\frac{\sigma(\gamma)}\gamma\]
	to give $S_{\alpha,\sigma} x=\cdot S_{\alpha',\sigma}$, where $S_{\alpha,\sigma}$ is the set of possible $\eta_\sigma$ defined in \autoref{cor:updatealpha}.

	We now proceed directly with the proof. Suppose that we have some triple $(\alpha_1,\alpha_2,\beta)\in T_\alpha$, which we know that we can write down as
	\[(\alpha_1,\alpha_2,\beta)=\left(\alpha\cdot\prod_{i=0}^{f-1}\sigma_K^i\left(\eta_{\sigma_K}\right),\quad\prod_{i=0}^{\varphi\left(p^\nu\right)-1}\sigma_x^i\left(\eta_{\sigma_x}\right),\quad\frac{\sigma_K\left(\eta_{\sigma_x}\right)}{\eta_{\sigma_x}}\cdot\frac{\eta_{\sigma_K}}{\sigma_x\left(\eta_{\sigma_K}\right)}\right)\]
	for some $\eta_{\sigma_K}\in S_{\alpha,\sigma_K}$ and $\eta_{\sigma_x}\in S_{\alpha,\sigma_x}$. We need to show that $(\alpha_1,\alpha_2,\beta)\in T_{\alpha'}$. Well, by \autoref{cor:updatealpha}, we can set
	\[I'_{\sigma}\coloneqq \eta_{\sigma}/\chi_\sigma\in S_{\alpha',\sigma}\]
	for $\sigma\in\{\sigma_K,\sigma_x\}$. We now compute
	\begin{align*}
		\alpha_1 ={}& \alpha\cdot\prod_{i=0}^{f-1}\sigma_K^i(\eta_{\sigma_K}) \\
		={}& \alpha\cdot\prod_{i=0}^{f-1}\sigma_K^i(\chi_\sigma)\cdot\prod_{i=0}^{f-1}\sigma_K^i(\eta_{\sigma_K'}) \\
		={}& \alpha\cdot\prod_{i=0}^{f-1}\sigma_K^i\left(\frac{\sigma_K\gamma}{\gamma}\right)\cdot\prod_{i=0}^{f-1}\sigma_K^i(\eta_{\sigma_K'}) \\
		={}& \alpha\cdot\frac{\sigma_K^f(\gamma)}{\gamma}\cdot\prod_{i=0}^{f-1}\sigma_K^i(\eta_{\sigma_K'}) \\
		={}& \alpha'\cdot\prod_{i=0}^{f-1}\sigma_K^i(\eta_{\sigma_K'}),
	\end{align*}
	where the last equality holds by definition of $\gamma$. Similarly, we see
	\begin{align*}
		\alpha_2 ={}& \prod_{i=0}^{\varphi\left(p^\nu\right)-1}\sigma_x^i(\eta_{\sigma_x}) \\
		={}& \prod_{i=0}^{\varphi\left(p^\nu\right)-1}\sigma_x^i(\chi_{\sigma_x})\cdot\prod_{i=0}^{\varphi\left(p^\nu\right)-1}\sigma_x^i(\eta_{\sigma_x}') \\
		={}& \prod_{i=0}^{\varphi\left(p^\nu\right)-1}\sigma_x^i\left(\frac{\sigma_x(\gamma)}{\gamma}\right)\cdot\prod_{i=0}^{\varphi\left(p^\nu\right)-1}\sigma_x^i(\eta_{\sigma_x}') \\
		={}& \prod_{i=0}^{\varphi\left(p^\nu\right)-1}\sigma_x^i(\eta_{\sigma_x}'),
	\end{align*}
	where the product telescopes in the last equality because $\sigma_x$ has order $\varphi\left(p^\nu\right)$. Lastly, we set
	\begin{align*}
		\beta &= \frac{\sigma_K\left(\eta_{\sigma_x}\right)}{\eta_{\sigma_x}}\cdot\frac{\eta_{\sigma_K}}{\sigma_x\left(\eta_{\sigma_K}\right)} \\
		&= \frac{\sigma_K\left(\chi_{\sigma_x}\right)}{\chi_{\sigma_x}}\cdot\frac{\chi_{\sigma_K}}{\sigma_x\left(\chi_{\sigma_K}\right)}\cdot\frac{\sigma_K\left(\eta_{\sigma_x}'\right)}{\eta_{\sigma_x}'}\cdot\frac{\eta_{\sigma_K}'}{\sigma_x\left(\eta_{\sigma_K}'\right)} \\
		&= \frac{\sigma_K\sigma_x\gamma/\sigma_K\gamma}{\sigma_x\gamma/\gamma}\cdot\frac{\sigma_K\gamma/\gamma}{\sigma_x\sigma_K\gamma/\sigma_x\gamma}\cdot\frac{\sigma_K\left(\eta_{\sigma_x}'\right)}{\eta_{\sigma_x}'}\cdot\frac{\eta_{\sigma_K}'}{\sigma_x\left(\eta_{\sigma_K}'\right)} \\
		&= \frac{\sigma_K\left(\eta_{\sigma_x}'\right)}{\eta_{\sigma_x}'}\cdot\frac{\eta_{\sigma_K}'}{\sigma_x\left(\eta_{\sigma_K}'\right)}.
	\end{align*}
	Thus,
	\[(\alpha_1,\alpha_2,\beta)=\left(\alpha'\cdot\prod_{i=0}^{f-1}\sigma_K^i\left(\eta_{\sigma_K}'\right),\quad\prod_{i=0}^{\varphi\left(p^\nu\right)-1}\sigma_x^i\left(\eta_{\sigma_x}'\right),\quad\frac{\sigma_K\left(\eta_{\sigma_x}'\right)}{\eta_{\sigma_x}'}\cdot\frac{\eta_{\sigma_K}'}{\sigma_x\left(\eta_{\sigma_K}'\right)}\right)\in T_{\alpha'},\]
	which finishes.
\end{proof}